src/spec/Flutterbye.Seq.Filter.fst
@@ -19,7 +19,7 @@
 module Flutterbye.Seq.Filter
 open FStar.Seq
 open Flutterbye.Seq.Mem
-open Flutterbye.Seq.Satisfies
+open Flutterbye.Seq.Contains
 
 // todo: ordering?
 // todo: counting?
@@ -37,7 +37,7 @@ type not_longer_than_p (#a_t:Type) (f:(a_t -> Tot bool)) (s:seq a_t) (s':seq a_t
 type when_nothing_satisfies_p (#a_t:Type) (f:(a_t -> Tot bool)) (s:seq a_t) (s':seq a_t) =
    (
        (length s' = 0)
-   //<==> (not (satisfies f s))
+   //<==> (not (contains f s))
    ==> (forall (x:nat{x < length s}).
           not (f (index s x)))
    )
@@ -59,17 +59,17 @@ type shared_membership_p (#a_t:Type) (f:(a_t -> Tot bool)) (s:seq a_t) (s':seq a
    )
 
 type filtered_p (#a_t:Type) (f:(a_t -> Tot bool)) (s:seq a_t) (s':seq a_t) =
-      empty_source_p f s s' 
+      empty_source_p f s s'
    /\ not_longer_than_p f s s'
    /\ everything_satisfies_p f s s'
    /\ shared_membership_p f s s'
    /\ when_nothing_satisfies_p f s s'
 
 private val filter_loop:
-      f:('a -> Tot bool) 
-   -> s:seq 'a 
-   -> i:nat{i <= length s} 
-   -> ac:seq 'a 
+      f:('a -> Tot bool)
+   -> s:seq 'a
+   -> i:nat{i <= length s}
+   -> ac:seq 'a
    -> Tot (ac':seq 'a)
       (decreases (length s - i))
 let rec filter_loop f s i ac =
@@ -85,10 +85,10 @@ let rec filter_loop f s i ac =
       ac
 
 private val filter_loop_lemma:
-      f:('a -> Tot bool) 
-   -> s:seq 'a 
-   -> i:nat{i <= length s} 
-   -> ac:seq 'a 
+      f:('a -> Tot bool)
+   -> s:seq 'a
+   -> i:nat{i <= length s}
+   -> ac:seq 'a
    -> Lemma
       (requires (filtered_p f (slice s 0 i) ac))
       (ensures (filtered_p f s (filter_loop f s i ac)))
